src/Lean/Meta/Tactic/Grind/Arith/Cutsat/Inv.lean
@@ -17,11 +17,10 @@ end Int.Linear
 
 namespace Lean.Meta.Grind.Arith.Cutsat
 
-def checkRelCnstrs (css : PArray (PArray RelCnstrWithProof)) (isLower : Bool) : GoalM Unit := do
+def checkLeCnstrs (css : PArray (PArray LeCnstr)) (isLower : Bool) : GoalM Unit := do
   let mut x := 0
   for cs in css do
-    for { c, .. } in cs do
-      assert! c.isLe
+    for c in cs do
       assert! c.isSorted
       assert! c.p.checkCoeffs
       let .add a y _ := c.p | unreachable!
@@ -33,22 +32,22 @@ def checkRelCnstrs (css : PArray (PArray RelCnstrWithProof)) (isLower : Bool) : 
 def checkLowers : GoalM Unit := do
   let s ← get'
   assert! s.lowers.size == s.vars.size
-  checkRelCnstrs s.lowers (isLower := true)
+  checkLeCnstrs s.lowers (isLower := true)
 
 def checkUppers : GoalM Unit := do
   let s ← get'
   assert! s.uppers.size == s.vars.size
-  checkRelCnstrs s.uppers (isLower := false)
+  checkLeCnstrs s.uppers (isLower := false)
 
 def checkDvdCnstrs : GoalM Unit := do
   let s ← get'
   assert! s.vars.size == s.dvdCnstrs.size
   let mut x := 0
   for c? in s.dvdCnstrs do
-    if let some { c, .. } := c? then
+    if let some c := c? then
       assert! c.p.checkCoeffs
       assert! c.p.isSorted
-      assert! c.k > 1
+      assert! c.d > 1
       let .add _ y _ := c.p | unreachable!
       assert! x == y
     x := x + 1
